Switch to ipda locale. Continue 2 ==> 3 proof

Escallon/LR_Parsing/Item_Pushdown_Automata.thy
@@ -4,28 +4,11 @@ theory Item_Pushdown_Automata
     Pushdown_Automata.Pushdown_Automata
 begin
 
- (* Better? *)
-(* locale ipda = Extended_Cfg G for G :: "('n::fresh0, 't) Cfg" +
-  fixes M :: "(('n, 't) item, 't, ('n, 't) item) pda"
-  assumes init_state:   "init_state M = [S' \<rightarrow> [] . [Nt S]]"
-      and init_symbol:  "init_symbol M = [S' \<rightarrow> [] . []]"
-      and final_states: "final_states M = {[S' \<rightarrow> [Nt S] . []]}"
-      and delta:        "delta M = (\<lambda>q a s. case q of [X \<rightarrow> \<beta> . Tm a' # \<gamma>] \<Rightarrow> 
-           if a' = a then let r = [X \<rightarrow> \<beta> @ [Tm a] . \<gamma>] in {(r, [s])} else {} | _ \<Rightarrow> {})"
-      and delta_eps:    "delta_eps M = (\<lambda>q s. case (q,s) of 
-      ([X \<rightarrow> \<beta> . Nt Y # \<gamma>], _) \<Rightarrow> {([Y \<rightarrow> [] . \<alpha>], [X \<rightarrow> \<beta> . Nt Y#\<gamma>]#[s]) |\<alpha>. (Y,\<alpha>) \<in> Prods G'} |
-      ([Y \<rightarrow> \<alpha> . []], [X \<rightarrow> \<beta> . Nt Y' # \<gamma>]) 
-        \<Rightarrow> if Y = Y' then {([X \<rightarrow> \<beta>@[Nt Y] . \<gamma>], [])} else {} | _ \<Rightarrow> {})" *)
 
-
-
-context Extended_Cfg
-begin
-
-definition IPDA :: "(('n, 't) item, 't, ('n, 't) item) pda" where
+definition (in Extended_Cfg) IPDA :: "(('n, 't) item, 't, ('n, 't) item) pda" where
   "IPDA \<equiv> let
     P = Prods G';
-    \<delta> = (\<lambda>q a s. case q of [X \<rightarrow> \<beta> . Tm a' # \<gamma>] \<Rightarrow> 
+    \<Delta> = (\<lambda>q a s. case q of [X \<rightarrow> \<beta> . Tm a' # \<gamma>] \<Rightarrow> 
             if a' = a then let r = [X \<rightarrow> \<beta> @ [Tm a] . \<gamma>] in {(r, [s])} else {} | _ \<Rightarrow> {});
     \<E> = (\<lambda>q s. case (q,s) of 
       ([X \<rightarrow> \<beta> . Nt Y # \<gamma>], _) \<Rightarrow> {([Y \<rightarrow> [] . \<alpha>], [X \<rightarrow> \<beta> . Nt Y#\<gamma>]#[s]) |\<alpha>. (Y,\<alpha>) \<in> P} |
@@ -33,40 +16,49 @@ definition IPDA :: "(('n, 't) item, 't, ('n, 't) item) pda" where
         \<Rightarrow> if Y = Y' then {([X \<rightarrow> \<beta>@[Nt Y] . \<gamma>], [])} else {} | _ \<Rightarrow> {})         
 in
   \<lparr>init_state = [S' \<rightarrow> [] . [Nt S]], init_symbol = [S' \<rightarrow> [] . []], 
-    final_states = {[S' \<rightarrow> [Nt S] . []]}, delta = \<delta>, delta_eps = \<E>\<rparr>"
+    final_states = {[S' \<rightarrow> [Nt S] . []]}, delta = \<Delta>, delta_eps = \<E>\<rparr>"
 
-lemma init_state_IPDA [simp]:
-  "init_state IPDA = [S' \<rightarrow> [] . [Nt S]]"
-  unfolding IPDA_def by simp
 
-lemma init_symbol_IPDA [simp]:
-  "init_symbol IPDA = [S' \<rightarrow> [] . []]"
-  unfolding IPDA_def by simp
+locale ipda = Extended_Cfg G for G :: "('n::fresh0, 't) Cfg" +
+  fixes M :: "(('n, 't) item, 't, ('n, 't) item) pda"
+  assumes ipda: "M = Extended_Cfg.IPDA G"
+begin
 
-lemma final_states_IPDA [simp]:
-  "final_states IPDA = {[S' \<rightarrow> [Nt S] . []]}"
-  unfolding IPDA_def by simp
 
-lemma delta_IPDA [simp]:
-  "delta IPDA = (\<lambda>q a s. case q of [X \<rightarrow> \<beta> . Tm a' # \<gamma>] \<Rightarrow> 
+lemma init_state_ipda [simp]:
+  "init_state M = [S' \<rightarrow> [] . [Nt S]]"
+  using ipda unfolding IPDA_def by simp
+
+lemma init_symbol_ipda [simp]:
+  "init_symbol M = [S' \<rightarrow> [] . []]"
+  using ipda unfolding IPDA_def by simp
+
+abbreviation "final_state \<equiv> [S' \<rightarrow> [Nt S] . []]"
+
+lemma final_states_ipda [simp]:
+  "final_states M = {final_state}"
+  using ipda unfolding IPDA_def by simp
+
+lemma delta_ipda [simp]:
+  "delta M = (\<lambda>q a s. case q of [X \<rightarrow> \<beta> . Tm a' # \<gamma>] \<Rightarrow> 
             if a' = a then let r = [X \<rightarrow> \<beta> @ [Tm a] . \<gamma>] in {(r, [s])} else {} | _ \<Rightarrow> {})"
-  unfolding IPDA_def by auto
+using ipda unfolding IPDA_def by simp
 
-lemma delta_eps_IPDA [simp]:
-  "delta_eps IPDA = (\<lambda>q s. case (q,s) of 
+lemma delta_eps_ipda [simp]:
+  "delta_eps M = (\<lambda>q s. case (q,s) of 
       ([X \<rightarrow> \<beta> . Nt Y # \<gamma>], _) \<Rightarrow> {([Y \<rightarrow> [] . \<alpha>], [X \<rightarrow> \<beta> . Nt Y#\<gamma>]#[s]) |\<alpha>. (Y,\<alpha>) \<in> Prods G'} |
       ([Y \<rightarrow> \<alpha> . []], [X \<rightarrow> \<beta> . Nt Y' # \<gamma>]) 
         \<Rightarrow> if Y = Y' then {([X \<rightarrow> \<beta>@[Nt Y] . \<gamma>], [])} else {} | _ \<Rightarrow> {})"
-  unfolding IPDA_def by simp
+  using ipda unfolding IPDA_def by simp
 
 
 lemma delta_Tm_neq_empty [simp]:
   assumes "a \<noteq> b"
-  shows "delta IPDA ([X \<rightarrow> \<alpha> . Tm a # \<gamma>]) b q = {}"
+  shows "delta M ([X \<rightarrow> \<alpha> . Tm a # \<gamma>]) b q = {}"
   using assms unfolding IPDA_def by simp
 
 lemma delta_nempty_impl_Tm_eq:
-  assumes "delta IPDA p a q \<noteq> {}"
+  assumes "delta M p a q \<noteq> {}"
   obtains X \<beta> \<gamma> where "p = [X \<rightarrow> \<beta> . Tm a # \<gamma>]"
 proof -
   obtain X \<beta> \<alpha> where p_def: "p = [X \<rightarrow> \<beta> . \<alpha>]" using item.exhaust by blast
@@ -78,12 +70,12 @@ qed
 
 lemma delta_eps_Nt_neq_empty [simp]:
   assumes "Y \<noteq> Y'"
-  shows "delta_eps IPDA ([Y \<rightarrow> \<alpha> . []]) ([X \<rightarrow> \<beta> . Nt Y' # \<gamma>]) = {}"
+  shows "delta_eps M ([Y \<rightarrow> \<alpha> . []]) ([X \<rightarrow> \<beta> . Nt Y' # \<gamma>]) = {}"
   using assms unfolding IPDA_def by simp
 
 
 lemma delta_eps_complete_impl_reducing:
-  assumes "delta_eps IPDA ([Y \<rightarrow> \<alpha> . []]) q \<noteq> {}"
+  assumes "delta_eps M ([Y \<rightarrow> \<alpha> . []]) q \<noteq> {}"
   obtains X \<beta> \<gamma> where "q = [X \<rightarrow> \<beta> . Nt Y # \<gamma>]"
 proof -
   obtain X \<beta> \<gamma> where q_def: "q = [X \<rightarrow> \<beta> . \<gamma>]" using item.exhaust by metis
@@ -96,7 +88,7 @@ proof -
 qed
 
 lemma delta_eps_nempty_impl_expanding_or_reducing:
-  assumes "delta_eps IPDA p q \<noteq> {}"
+  assumes "delta_eps M p q \<noteq> {}"
   obtains X \<beta> Y \<gamma> where "p = [X \<rightarrow> \<beta> . Nt Y # \<gamma>]"  |
     Y \<alpha> X \<beta>  \<gamma> where "p = [Y \<rightarrow> \<alpha> . []]" "q = [X \<rightarrow> \<beta> . Nt Y # \<gamma>]"
 proof -
@@ -113,59 +105,38 @@ proof -
   qed
 qed
 
-
-type_synonym ('q,'s) ipda_config = "'q list \<times> 's list"
-
 lemmas init_defs = init_state_def init_symbol_def
 
-abbreviation "final_state \<equiv> [S' \<rightarrow> [Nt S] . []]"
-
 lemma in_final_impl_final_state:
-  assumes "q \<in> final_states IPDA"
+  assumes "q \<in> final_states M"
   shows "q = final_state"
   using assms unfolding IPDA_def S'_def S_def by simp
 
-lemma final_state_in_final[simp]:
-  "final_state \<in> final_states IPDA"
-  unfolding IPDA_def S'_def S_def by simp
+inductive step :: "('n,'t) item list \<times> 't list \<Rightarrow> ('n,'t) item list \<times> 't list 
+                    \<Rightarrow> bool" (infix \<open>\<turnstile>\<close> 70) where
+delta[intro]: "\<lbrakk>\<alpha> = [p0, p1]; \<alpha>' = q#qs; (q,qs) \<in> delta M p0 a p1\<rbrakk> 
+                \<Longrightarrow> (\<alpha>@\<beta>,a#w) \<turnstile> (\<alpha>'@\<beta>,w)" |
+eps[intro]: "\<lbrakk>\<alpha> = [p0, p1]; \<alpha>' = q#qs; (q,qs) \<in> delta_eps M p0 p1\<rbrakk> 
+                \<Longrightarrow> (\<alpha>@\<beta>, w) \<turnstile> (\<alpha>'@\<beta>, w)"
 
-
-
-lemma delta_init_empty:
-  "delta IPDA (init_state IPDA) a (init_symbol IPDA) = {}"
-proof -
-  let ?\<delta> = "(\<lambda>q a s. case q of [X \<rightarrow> \<beta> . Tm a' # \<gamma>] \<Rightarrow> 
-            if a' = a then let r = [X \<rightarrow> \<beta> @ [Tm a] . \<gamma>] in {(r, [s])} else {} | _ \<Rightarrow> {})"
-  have delta: "?\<delta> = delta IPDA"  unfolding IPDA_def by simp
-  from init_state_def have "?\<delta> (init_state IPDA) a (init_symbol IPDA) = {}" 
-    by auto
-  with ext delta show ?thesis  by (metis (lifting))
-qed
-
-inductive step :: "(('n,'t) item,'t) ipda_config \<Rightarrow> (('n,'t) item,'t) ipda_config \<Rightarrow> bool" (infix \<open>\<turnstile>P\<close> 70) where
-delta[intro]: "\<lbrakk>\<alpha> = [p0, p1]; \<alpha>' = q#qs; (q,qs) \<in> delta IPDA p0 a p1\<rbrakk> 
-                \<Longrightarrow> (\<alpha>@\<beta>,a#w) \<turnstile>P (\<alpha>'@\<beta>,w)" |
-eps[intro]: "\<lbrakk>\<alpha> = [p0, p1]; \<alpha>' = q#qs; (q,qs) \<in> delta_eps IPDA p0 p1\<rbrakk> 
-                \<Longrightarrow> (\<alpha>@\<beta>, w) \<turnstile>P (\<alpha>'@\<beta>, w)"
-
-inductive_cases step_deltaE[elim]: "(s, x#w) \<turnstile>P (s', w)"
-inductive_cases step_epsE[elim]: "(s, w) \<turnstile>P (s', w)"
+inductive_cases step_deltaE[elim]: "(s, x#w) \<turnstile> (s', w)"
+inductive_cases step_epsE[elim]: "(s, w) \<turnstile> (s', w)"
 
 lemma step_equal_or_Cons:
-  assumes "(p,u) \<turnstile>P (q,v)"
+  assumes "(p,u) \<turnstile> (q,v)"
   shows "u = v \<or> (\<exists>a. u = a#v)"
   using assms by cases auto
 
 lemma step_len_dec:
-  assumes "(p,u) \<turnstile>P (q,v)"
+  assumes "(p,u) \<turnstile> (q,v)"
   shows "length u \<ge> length v" 
   using step_equal_or_Cons[OF assms] by fastforce
 
 
 lemma shifting[simp]:
-  "([A \<rightarrow> \<alpha> . Tm a # \<beta>]#\<rho>#\<rho>s, a#u) \<turnstile>P ([A \<rightarrow> \<alpha>@[Tm a] . \<beta>]#\<rho>#\<rho>s, u)"
+  "([A \<rightarrow> \<alpha> . Tm a # \<beta>]#\<rho>#\<rho>s, a#u) \<turnstile> ([A \<rightarrow> \<alpha>@[Tm a] . \<beta>]#\<rho>#\<rho>s, u)"
 proof -
-  have "([A \<rightarrow> \<alpha>@[Tm a] . \<beta>], [\<rho>]) \<in> delta IPDA ([A \<rightarrow> \<alpha> . Tm a # \<beta>]) a \<rho>"
+  have "([A \<rightarrow> \<alpha>@[Tm a] . \<beta>], [\<rho>]) \<in> delta M ([A \<rightarrow> \<alpha> . Tm a # \<beta>]) a \<rho>"
     using IPDA_def by simp
   then show ?thesis using delta 
     by (metis Cons_eq_appendI append.left_neutral)
@@ -173,54 +144,44 @@ qed
 
 
 lemma reducing[simp]:
-  "([Y \<rightarrow> \<alpha> . []]#[X \<rightarrow> \<beta> . Nt Y#\<gamma>]#\<rho>, w) \<turnstile>P ([X \<rightarrow> \<beta> @ [Nt Y] . \<gamma>]#\<rho>, w)"
+  "([Y \<rightarrow> \<alpha> . []]#[X \<rightarrow> \<beta> . Nt Y#\<gamma>]#\<rho>, w) \<turnstile> ([X \<rightarrow> \<beta> @ [Nt Y] . \<gamma>]#\<rho>, w)"
 proof -
-  have "([X \<rightarrow> \<beta> @ [Nt Y] . \<gamma>], []) \<in> delta_eps IPDA ([Y \<rightarrow> \<alpha> . []]) ([X \<rightarrow> \<beta> . Nt Y#\<gamma>])"
+  have "([X \<rightarrow> \<beta> @ [Nt Y] . \<gamma>], []) \<in> delta_eps M ([Y \<rightarrow> \<alpha> . []]) ([X \<rightarrow> \<beta> . Nt Y#\<gamma>])"
     unfolding IPDA_def by simp
   thus ?thesis using eps by (metis Cons_eq_appendI append.left_neutral)
 qed
 
 lemma expanding_in_delta_eps:
   assumes "(Y, \<alpha>) \<in> Prods G'"
-  shows "([Y \<rightarrow> [] . \<alpha>], [[X \<rightarrow> \<beta> . Nt Y#\<gamma>], i]) \<in> delta_eps IPDA ([X \<rightarrow> \<beta> . Nt Y#\<gamma>]) i"
-  using assms unfolding G'_def S'_def S_def IPDA_def by auto
+  shows "([Y \<rightarrow> [] . \<alpha>], [[X \<rightarrow> \<beta> . Nt Y#\<gamma>], i]) \<in> delta_eps M ([X \<rightarrow> \<beta> . Nt Y#\<gamma>]) i"
+  using assms ipda unfolding G'_def S'_def S_def IPDA_def by auto
 
 lemma expanding[simp]:
   assumes "(Y, \<alpha>) \<in> Prods G'"
-  shows "([X \<rightarrow> \<beta> . Nt Y#\<gamma>]#i#\<rho>, w) \<turnstile>P ([Y \<rightarrow> [] . \<alpha>]#[X \<rightarrow> \<beta> . Nt Y#\<gamma>]#i#\<rho>, w)"
+  shows "([X \<rightarrow> \<beta> . Nt Y#\<gamma>]#i#\<rho>, w) \<turnstile> ([Y \<rightarrow> [] . \<alpha>]#[X \<rightarrow> \<beta> . Nt Y#\<gamma>]#i#\<rho>, w)"
   using expanding_in_delta_eps[OF assms] eps 
   by (metis eq_Nil_appendI Cons_eq_appendI)
 
 lemma in_delta_impl_shifting:
-  assumes "(q, qs) \<in> delta IPDA p0 a p1"
+  assumes "(q, qs) \<in> delta M p0 a p1"
   obtains X \<beta> \<gamma> where "p0 = [X \<rightarrow> \<beta> . Tm a # \<gamma>]"
     "(q,qs) = ([X \<rightarrow> \<beta> @ [Tm a] . \<gamma>], [p1])"
 proof -
-  from assms have nempty: "delta IPDA p0 a p1 \<noteq> {}" by auto
-  let ?\<delta> = "(\<lambda>q a s. case q of [X \<rightarrow> \<beta> . Tm a' # \<gamma>] \<Rightarrow> 
-            if a' = a then let r = [X \<rightarrow> \<beta> @ [Tm a] . \<gamma>] in {(r, [s])} else {} | _ \<Rightarrow> {})"
-  have \<delta>_def: "?\<delta> = delta IPDA" unfolding IPDA_def by simp
-  from delta_nempty_impl_Tm_eq[OF nempty] 
-    obtain X \<beta> \<gamma> where p0_def: "p0 = [X \<rightarrow> \<beta> . Tm a # \<gamma>]" 
-    by blast
-  hence "?\<delta> p0 a p1 = {([X \<rightarrow> \<beta> @ [Tm a] . \<gamma>], [p1])}" by simp
-  with assms show thesis using \<delta>_def that p0_def 
+  from assms have "delta M p0 a p1 \<noteq> {}" by auto
+  from delta_nempty_impl_Tm_eq[OF this] 
+    obtain X \<beta> \<gamma> where p0_def: "p0 = [X \<rightarrow> \<beta> . Tm a # \<gamma>]" by blast
+  hence "delta M p0 a p1 = {([X \<rightarrow> \<beta> @ [Tm a] . \<gamma>], [p1])}" by simp
+  with assms show thesis using delta_ipda that p0_def 
     by (metis (lifting) singletonD)
 qed
 
 lemma eps_cases[consumes 1, case_names reducing expanding]:
-  assumes "(q0,qs) \<in> delta_eps IPDA p0 p1"
+  assumes "(q0,qs) \<in> delta_eps M p0 p1"
   obtains Y \<alpha> X \<beta> \<gamma> where
     "p0 = [Y \<rightarrow> \<alpha> . []]" "p1 = [X \<rightarrow> \<beta> . Nt Y # \<gamma>]" "q0 = [X \<rightarrow> \<beta> @ [Nt Y] . \<gamma>]" "qs = []" |
     X \<beta> Y \<gamma> \<alpha> where
     "p0 = [X \<rightarrow> \<beta> . Nt Y # \<gamma>]" "(Y, \<alpha>) \<in> Prods G'" "q0 = [Y \<rightarrow> [] . \<alpha>]" "qs = p0#[p1]" 
 proof -
-  let ?\<delta> = "(\<lambda>q s. case (q,s) of 
-      ([X \<rightarrow> \<beta> . Nt Y # \<gamma>], _) \<Rightarrow> {([Y \<rightarrow> [] . \<alpha>], [X \<rightarrow> \<beta> . Nt Y#\<gamma>]#[s]) |\<alpha>. (Y,\<alpha>) \<in> Prods G'} |
-      ([Y \<rightarrow> \<alpha> . []], [X \<rightarrow> \<beta> . Nt Y' # \<gamma>]) 
-        \<Rightarrow> if Y = Y' then {([X \<rightarrow> \<beta>@[Nt Y] . \<gamma>], [])} else {} | _ \<Rightarrow> {})"
-  have "delta_eps IPDA = ?\<delta>"
-    using delta_eps_IPDA S_def S'_def G'_def by fastforce
   from delta_eps_nempty_impl_expanding_or_reducing consider 
     X \<beta> Y \<gamma> where "p0 = [X \<rightarrow> \<beta> . Nt Y # \<gamma>]" |
     Y \<alpha> X \<beta> \<gamma> where "p0 = [Y \<rightarrow> \<alpha> . []]" "p1 = [X \<rightarrow> \<beta> . Nt Y # \<gamma>]" 
@@ -230,7 +191,7 @@ proof -
 qed
 
 lemma step_cases[consumes 1, case_names shifting reducing expanding]:
-  assumes "c0 \<turnstile>P c1"
+  assumes "c0 \<turnstile> c1"
 obtains A \<alpha> a \<beta> i \<rho> u where 
     "c0 = ([A \<rightarrow> \<alpha> . Tm a # \<beta>]#i#\<rho>, a#u)" "c1 = ([A \<rightarrow> \<alpha>@[Tm a] . \<beta>]#i#\<rho>, u)" |
     Y \<alpha> X \<beta> \<gamma> \<rho> w where
@@ -240,75 +201,57 @@ obtains A \<alpha> a \<beta> i \<rho> u where
       "(Y, \<alpha>) \<in> Prods G'"
   using assms proof cases
   case (delta \<alpha> p0 p1 \<alpha>' q qs a \<beta> w)
-  thm IPDA_def
   from in_delta_impl_shifting[OF delta(5)] obtain X \<beta>' \<gamma> where "p0 = [X \<rightarrow> \<beta>' . Tm a # \<gamma>]" 
     "(q,qs) = ([X \<rightarrow> \<beta>' @ [Tm a] . \<gamma>], [p1])" by blast
   then show ?thesis using that delta by simp 
 next
   case (eps \<alpha> p0 p1 \<alpha>' q qs \<beta> w)
-  from eps(5) show ?thesis 
-    by (cases rule: eps_cases) 
-      (use expanding_in_delta_eps eps_cases eps that in force)+
+  from eps(5) expanding_in_delta_eps eps_cases eps that show ?thesis 
+    by (cases rule: eps_cases) force+
 qed
 
 lemma step_impl_in_It:
   assumes "i0 \<in> It G'" "i1 \<in> It G'"
-    "(i0#i1#is, u) \<turnstile>P (j#js, v)"
+    "(i0#i1#is, u) \<turnstile> (j#js, v)"
   shows "j \<in> It G'"
-using assms(3) proof (cases rule: step_cases)
-  case (shifting A \<alpha> a \<beta> i \<rho> u)
-  then show ?thesis using assms(1) unfolding It_defs by simp
-next
-  case (reducing Y \<alpha> X \<beta> \<gamma> \<rho> w)
-  then show ?thesis using assms(1,2) unfolding It_defs by simp
-next
-  case (expanding Y \<alpha> X \<beta> \<gamma> i \<rho> w)
-  then show ?thesis unfolding It_defs by simp
-qed
-  
+  using assms(3,1,2) by (cases rule: step_cases) (simp add: It_defs)+
 
 
-abbreviation steps (infix \<open>\<turnstile>P*\<close> 70) where
+abbreviation steps (infix \<open>\<turnstile>*\<close> 70) where
   "steps \<equiv> (step \<^sup>*\<^sup>*)"
 
-abbreviation stepn ( \<open>_ \<turnstile>P'(_') _\<close> 70) where
+abbreviation stepn ( \<open>_ \<turnstile>'(_') _\<close> 70) where
   "stepn c0 n c1 \<equiv> (step ^^ n) c0 c1"
 
 lemma steps_len_dec:
-  "(p,u) \<turnstile>P* (q,v) \<Longrightarrow> length u \<ge> length v" 
-  by ((induction "(p,u)" "(q,v)" arbitrary: q v rule: rtranclp.induct),
-  (use step_len_dec surj_pair le_trans in fastforce)+)
+  "(p,u) \<turnstile>* (q,v) \<Longrightarrow> length u \<ge> length v" 
+  by (induction "(p,u)" "(q,v)" arbitrary: q v rule: rtranclp.induct)
+  (use step_len_dec surj_pair le_trans in fastforce)+
 
 lemma syms_complete:
-  "([A \<rightarrow> \<alpha> . map Tm u @ \<beta>]#i#is, u@v) \<turnstile>P* ([A \<rightarrow> \<alpha> @ map Tm u . \<beta>]#i#is, v)"
+  "([A \<rightarrow> \<alpha> . map Tm u @ \<beta>]#i#is, u@v) \<turnstile>* ([A \<rightarrow> \<alpha> @ map Tm u . \<beta>]#i#is, v)"
 proof (induction u arbitrary: \<alpha>)
   case (Cons a u)
   have "([A \<rightarrow> \<alpha> . map Tm (a # u) @ \<beta>] # i # is, (a # u) @ v) 
-        \<turnstile>P ([A \<rightarrow> \<alpha> @ [Tm a] . map Tm u @ \<beta>] # i # is, u @ v)"
+        \<turnstile> ([A \<rightarrow> \<alpha> @ [Tm a] . map Tm u @ \<beta>] # i # is, u @ v)"
     by simp
   also note Cons[of "\<alpha>@[Tm a]"] 
   finally show ?case by auto
 qed simp
 
 lemma reachable_impl_in_It:
-  "\<lbrakk>([init_state IPDA, init_symbol IPDA], u) \<turnstile>P* (\<rho>1, v); i \<in> set \<rho>1 - {init_symbol IPDA}\<rbrakk> 
+  "\<lbrakk>([init_state M, init_symbol M], u) \<turnstile>* (\<rho>1, v); i \<in> set \<rho>1 - {init_symbol M}\<rbrakk> 
     \<Longrightarrow> i \<in> It G'"
 proof (induction arbitrary: i rule: rtranclp_induct2)
-  case refl
-  then show ?case unfolding It_defs G'_def by auto
-next
   case (step \<rho>0 u \<rho>1 v)
-  note step_unfolded = step(3,4)[unfolded It_defs]
   from step(2) show ?case 
-    (* Avoid apply? *)
-    apply (cases rule: step_cases)
-    using step(3,4) by (fastforce simp: It_defs(2))+
-qed
+    using step(3,4) by (cases rule: step_cases) (fastforce simp: It_defs)+ 
+qed (auto simp: It_defs G'_def)
 
 
 
 lemma steps_substring:
-  assumes "(\<rho>0, w) \<turnstile>P* (\<rho>2, v)"
+  assumes "(\<rho>0, w) \<turnstile>* (\<rho>2, v)"
   obtains u where "w = u@v"
   sorry
 
@@ -321,24 +264,24 @@ lemma list_app_last_is_next_hd:
   by (metis append.assoc append_Cons append_Nil append_same_eq last_append last_snoc)
 
 lemma reachable_impl_reachable_substring:
-  assumes "(\<rho>0, u) \<turnstile>P* (\<rho>2, y)"
+  assumes "(\<rho>0, u) \<turnstile>* (\<rho>2, y)"
     "u = v@w@y"
-  obtains \<rho>1 where "(\<rho>0, u) \<turnstile>P* (\<rho>1, w@y)"
+  obtains \<rho>1 where "(\<rho>0, u) \<turnstile>* (\<rho>1, w@y)"
 proof -
-  from assms(1) obtain n where "(\<rho>0, u) \<turnstile>P(n) (\<rho>2, y)"
+  from assms(1) obtain n where "(\<rho>0, u) \<turnstile>(n) (\<rho>2, y)"
     by (metis rtranclp_imp_relpowp)
-  with assms(2) obtain \<rho>1 where "(\<rho>0, u) \<turnstile>P* (\<rho>1, w@y)"
+  with assms(2) obtain \<rho>1 where "(\<rho>0, u) \<turnstile>* (\<rho>1, w@y)"
   proof (induction n arbitrary: \<rho>2 v w y thesis rule: less_induct)
     case (less n)
     show ?case 
     proof (cases n)
       case (Suc m)
-      with less(4) obtain \<rho>1 z where msteps: "(\<rho>0, u) \<turnstile>P(m) (\<rho>1, z)" "(\<rho>1, z) \<turnstile>P (\<rho>2, y)" by auto
+      with less(4) obtain \<rho>1 z where msteps: "(\<rho>0, u) \<turnstile>(m) (\<rho>1, z)" "(\<rho>1, z) \<turnstile> (\<rho>2, y)" by auto
       from msteps(2) consider "z = y" | a where "z = a#y" using step.cases by blast
       then show ?thesis
       proof cases
         case 1
-        with less(1,3) msteps(1) Suc obtain \<rho>' where "(\<rho>0, u) \<turnstile>P* (\<rho>', w @ y)" by blast
+        with less(1,3) msteps(1) Suc obtain \<rho>' where "(\<rho>0, u) \<turnstile>* (\<rho>', w @ y)" by blast
         then show ?thesis using less(2) by blast
       next
         case 2
@@ -351,7 +294,7 @@ proof -
             using as list_app_last_is_next_hd[OF less(3)] 
             by (metis list.distinct(1) snoc_eq_iff_butlast)
           hence "u = v @ cs @ z" using less 2 by simp
-          from less(1)[OF _ _ this msteps(1)] obtain \<rho>' where "(\<rho>0, u) \<turnstile>P* (\<rho>', cs @ z)"
+          from less(1)[OF _ _ this msteps(1)] obtain \<rho>' where "(\<rho>0, u) \<turnstile>* (\<rho>', cs @ z)"
             using Suc by blast
           then show ?thesis using cs_def 2 less(2) by simp
         qed (use less rtranclp_power append_Nil in metis)
@@ -363,78 +306,87 @@ qed
 
 
 lemma syms_tl_impl_substring:
-  assumes "([A \<rightarrow> \<alpha> . \<beta> @ map Tm u]#\<rho>, v) \<turnstile>P* ([A \<rightarrow> \<alpha>@\<beta>@map Tm u . []]#\<rho>', w)"
+  assumes "([A \<rightarrow> \<alpha> . \<beta> @ map Tm u]#\<rho>, v) \<turnstile>* ([A \<rightarrow> \<alpha>@\<beta>@map Tm u . []]#\<rho>', w)"
   obtains v' where "v = v'@u"
   sorry
 
 lemma reaches_final_impl_reaches_complete:
-  assumes "([A \<rightarrow> \<alpha> . \<beta>]#\<rho>, v) \<turnstile>P* ([[S' \<rightarrow> [Nt S] . []], init_symbol IPDA], [])"
-  obtains w where "([A \<rightarrow> \<alpha> . \<beta>]#\<rho>, v) \<turnstile>P* ([A \<rightarrow> \<alpha>@\<beta> . []]#\<rho>', w)"
+  assumes "([A \<rightarrow> \<alpha> . \<beta>]#\<rho>, v) \<turnstile>* ([final_state, init_symbol M], [])"
+  obtains w where "([A \<rightarrow> \<alpha> . \<beta>]#\<rho>, v) \<turnstile>* ([A \<rightarrow> \<alpha>@\<beta> . []]#\<rho>', w)"
   sorry
 
 corollary reaches_final_impl_substring:
-  assumes "([A \<rightarrow> \<alpha> . \<beta> @ map Tm u]#\<rho>, v) \<turnstile>P* ([[S' \<rightarrow> [Nt S] . []], init_symbol IPDA], [])"
+  assumes "([A \<rightarrow> \<alpha> . \<beta> @ map Tm u]#\<rho>, v) \<turnstile>* ([final_state, init_symbol M], [])"
   obtains v' where "v = v'@u"
   using reaches_final_impl_reaches_complete[OF assms, THEN syms_tl_impl_substring]
   by metis
 
 lemma reaches_final_impl_interm_reaches_final:
-  assumes "c0 \<turnstile>P* ([[S' \<rightarrow> [Nt S] . []], init_symbol IPDA], [])"
-    "c0 \<turnstile>P* c1"
-  shows "c1 \<turnstile>P* ([[S' \<rightarrow> [Nt S] . []], init_symbol IPDA], [])"
+  assumes "c0 \<turnstile>* ([final_state, init_symbol M], [])"
+    "c0 \<turnstile>* c1"
+  shows "c1 \<turnstile>* ([final_state, init_symbol M], [])"
   sorry
 
+lemma computes_impl_Nt_on_stack:
+  assumes "([init_state M, init_symbol M], u) \<turnstile>* ([A \<rightarrow> \<alpha> . \<beta>]#\<rho>@[init_symbol M], v)"
+    "A \<noteq> S'"
+  obtains B \<gamma> \<delta> js  where "\<rho> = [B \<rightarrow> \<gamma> . Nt A # \<delta>]#js"
+  using assms apply (induction rule: rtranclp_induct2) sorry
+
+lemma derives_impl_completes:
+   "Prods G' \<turnstile> \<beta> \<Rightarrow>* map Tm v \<Longrightarrow> ([A \<rightarrow> \<alpha> . \<beta>@\<gamma>]#\<rho>, v@w) \<turnstile>* ([A \<rightarrow> \<alpha>@\<beta> . \<gamma>]#\<rho>, w)"
+proof (induction \<beta> arbitrary: v)
+  case (Cons a \<beta>)
+  then show ?case 
+    apply (cases a)
+    sorry
+qed simp
 
 
-definition ipda_Lang :: "'t list set" where
-  "ipda_Lang \<equiv> {w. ([init_state IPDA, init_symbol IPDA], w)
-             \<turnstile>P* ([[S' \<rightarrow> [Nt S] . []], init_symbol IPDA], [])}"
+definition Lang :: "'t list set" where
+  "Lang \<equiv> {w. ([init_state M, init_symbol M], w)
+             \<turnstile>* ([final_state, init_symbol M], [])}"
 
 
 lemma hist_singleton_init [simp]:
-  "hist ([[A \<rightarrow> \<alpha> . \<beta>], init_symbol IPDA]) = \<alpha>"
+  "hist ([[A \<rightarrow> \<alpha> . \<beta>], init_symbol M]) = \<alpha>"
   unfolding IPDA_def using hist_singleton by auto
 
 lemma hist_init [simp]:
-  "hist (\<rho>@[init_symbol IPDA]) = hist \<rho>"
+  "hist (\<rho>@[init_symbol M]) = hist \<rho>"
   using IPDA_def by (induction \<rho>) auto
 
 lemma invariant: 
-  assumes "([init_state IPDA, init_symbol IPDA], u@v) \<turnstile>P* (\<rho>, v)"
+  assumes "([init_state M, init_symbol M], u@v) \<turnstile>* (\<rho>, v)"
   shows "Prods G \<turnstile> hist \<rho> \<Rightarrow>* map Tm u"
   sorry
 
-corollary ipda_Lang_subst_Lang_G:
-  "ipda_Lang \<subseteq> LangS G"
-  unfolding ipda_Lang_def Context_Free_Grammar.Lang_def S_def 
+corollary Lang_subst_Lang_G:
+  "Lang \<subseteq> LangS G"
+  unfolding Lang_def Context_Free_Grammar.Lang_def S_def 
   by (standard, metis invariant append.right_neutral hist_singleton_init mem_Collect_eq)
-
-lemma derives_impl_completes:
-  assumes "Prods G \<turnstile> [Nt A] \<Rightarrow> \<alpha>"
-    "Prods G \<turnstile> \<alpha> \<Rightarrow>* map Tm w"
-  shows "([A \<rightarrow> [] . \<alpha>]#\<rho>, w@v) \<turnstile>P* ([A \<rightarrow> \<alpha> . []]#\<rho>, v)"
-  sorry
+ 
 
 
-lemma ipda_Lang_eq_Lang_G:
-  "ipda_Lang = LangS G"
+lemma Lang_eq_Lang_G:
+  "Lang = LangS G"
   sorry
 
 
 lemma first_step_is_eps:
-  assumes "([init_state IPDA, init_symbol IPDA], u) \<turnstile>P* (qs, v)"
-    "([init_state IPDA, init_symbol IPDA], u) \<noteq> (qs, v)"
+  assumes "([init_state M, init_symbol M], u) \<turnstile>* (qs, v)"
+    "([init_state M, init_symbol M], u) \<noteq> (qs, v)"
   obtains \<alpha> where 
-    "([init_state IPDA, init_symbol IPDA], u) \<turnstile>P ([[S \<rightarrow> [] . \<alpha>], init_state IPDA, init_symbol IPDA], u)"
-    "([[S \<rightarrow> [] . \<alpha>], init_state IPDA, init_symbol IPDA], u) \<turnstile>P* (qs, v)"
+    "([init_state M, init_symbol M], u) \<turnstile> ([[S \<rightarrow> [] . \<alpha>], init_state M, init_symbol M], u)"
+    "([[S \<rightarrow> [] . \<alpha>], init_state M, init_symbol M], u) \<turnstile>* (qs, v)"
 proof -
-  from assms obtain ps u' where step: "([init_state IPDA, init_symbol IPDA], u) \<turnstile>P (ps, u')"
-    and steps: "(ps, u') \<turnstile>P* (qs, v)"
+  from assms obtain ps u' where step: "([init_state M, init_symbol M], u) \<turnstile> (ps, u')"
+    and steps: "(ps, u') \<turnstile>* (qs, v)"
     by (metis converse_rtranclpE2)
   moreover have "u = u'" 
-    by (rule ccontr, use step delta_init_empty step_equal_or_Cons in fastforce)
+    by (rule ccontr) (use step step_equal_or_Cons in fastforce)
   moreover with step obtain r rs where 
-    "ps = r#rs" "(r, rs) \<in> delta_eps IPDA (init_state IPDA) (init_symbol IPDA)"
+    "ps = r#rs" "(r, rs) \<in> delta_eps M (init_state M) (init_symbol M)"
     using step_epsE by fastforce 
   ultimately show thesis using that by auto
 qed
